Use strings in Coq and support break/continue natively.
We now use strings for names of structs/unions, goto labels, and function
names in the Coq part. Also in the frontend, we use strings for all names.

This has the following advantages:
* No need to rename in the Ocaml part. This makes the code better readable.
* Given C syntax in Coq, we can see easily trace where names came from.
* We can generate better error messages (remains to be done).

But also some disadvantages:
* Maps/sets with string indexes are potentially slower. We have implemented
  these using uncompressed Patricia trees, so it is not super bad (and this
  gives at least canonical representations), but these trees can become
  rather big.
* Generating fresh strings is annoying, but we only used that to generate
  names for labels of gotos for break/continue. These are now natively
  supported in the semantics.

Break and continue is now natively supported in the C semantics. We have
introduced the constructs

  break n
  breakto s

The construct break n breaks to the nth surrounding breakto.

parser/Main.ml
@@ -38,9 +38,6 @@ let rec positive_of_int n =
   let n' = positive_of_int (n/2) in
   if n mod 2 = 1 then XI n' else XO n';;
 
-let n_of_int n =
-  if n = 0 then N0 else Npos (positive_of_int n);;
-
 let z_of_int i =
   if i = 0 then Z0 else if i > 0 then Zpos (positive_of_int i) else
   Zneg (positive_of_int (-i));;
@@ -51,9 +48,6 @@ let rec int_of_nat n =
 let rec int_of_positive n =
   match n with XI n' -> 2*(int_of_positive n') + 1 |
     XO n' -> 2*(int_of_positive n') | XH -> 1;;
-
-let int_of_n n =
-  match n with N0 -> 0 | Npos n' -> int_of_positive n';;
 
 let int_of_z i =
   match i with Z0 -> 0 | Zpos n' -> int_of_positive n'
@@ -67,9 +61,6 @@ let rec positive_of_num n =
   let n' = positive_of_num (quo_num n (Int 2)) in
   if mod_num n (Int 2) = Int 1 then XI n' else XO n';;
 
-let n_of_num n =
-  if n = Int 0 then N0 else Npos (positive_of_num n);;
-
 let z_of_num i =
   if i = Int 0 then Z0 else if i >/ Int 0 then Zpos (positive_of_num i) else
   Zneg (positive_of_num (minus_num i));;
@@ -80,9 +71,6 @@ let rec num_of_nat n =
 let rec num_of_positive n =
   match n with XI n' -> Int 2*/(num_of_positive n') +/ Int 1 |
     XO n' -> Int 2*/(num_of_positive n') | XH -> Int 1;;
-
-let num_of_n n =
-  match n with N0 -> Int 0 | Npos n' -> num_of_positive n';;
 
 let num_of_z i =
   match i with Z0 -> Int 0 | Zpos n' -> num_of_positive n'
@@ -98,24 +86,6 @@ let pp_print_nat fmt x =
       pp_print_string fmt ")")
   | y ->
      (pp_print_string fmt "(nat_of_num";
-      pp_print_space fmt ();
-      pp_print_string fmt "(num_of_string";
-      pp_print_space fmt ();
-      pp_print_string fmt "\"";
-      pp_print_string fmt (string_of_num y);
-      pp_print_string fmt "\"))"));
-  pp_close_box fmt ();;
-
-let pp_print_n fmt x =
-  pp_open_box fmt 2;
- (match num_of_n x with
-  | Int y ->
-     (pp_print_string fmt "(n_of_int";
-      pp_print_space fmt ();
-      pp_print_int fmt y;
-      pp_print_string fmt ")")
-  | y ->
-     (pp_print_string fmt "(n_of_num";
       pp_print_space fmt ();
       pp_print_string fmt "(num_of_string";
       pp_print_space fmt ();
@@ -144,8 +114,6 @@ let pp_print_z fmt x =
 
 let print_nat = pp_print_nat std_formatter;;
 #install_printer print_nat;;
-let print_n = pp_print_n std_formatter;;
-#install_printer print_n;;
 let print_z = pp_print_z std_formatter;;
 #install_printer print_z;;
 
@@ -189,25 +157,19 @@ let chars_of_string s =
     if n < l then String.get s n::chars (n + 1) else [] in
   chars 0;;
 
+let chars_of_int n = chars_of_string (string_of_int n)
+
 exception Unknown_expression of Cabs.expression;;
 exception Unknown_statement of Cabs.statement;;
 exception Unknown_specifier of Cabs.specifier;;
 exception Unknown_definition of Cabs.definition;;
-exception Incompatible_compound of n * decl * decl;;
+exception Incompatible_compound of char list * decl * decl;;
 
 let col = ref 0;;
-let the_ids = ref ([]:string list);;
 let the_anon = ref 0;;
-let the_compound_decls = ref ([]:(n * decl) list);;
-let the_printfs = ref ([]:(n * decl) list);;
-let the_formats = ref ([]:(n * string) list);;
-
-let nindex s =
-  n_of_int (try index s !the_ids with
-  Not_found ->
-    let ids = !the_ids in
-    the_ids := ids@[s];
-    List.length ids);;
+let the_compound_decls = ref ([]:(char list * decl) list);;
+let the_printfs = ref ([]:(char list * decl) list);;
+let the_formats = ref ([]:(char list * string) list);;
 
 let uchar = {csign = Some Unsigned; crank = CCharRank};;
 let int_signed = {csign = Some Signed; crank = CIntRank};;
@@ -276,18 +238,18 @@ let length_of_format s =
   length 0;;
 
 let printf_body i =
-  let len = nindex "len-%d" in
+  let len = chars_of_string "len-%d" in
   let rec body n a =
     match a with
     | [] -> CSReturn (Some (CEVar i))
     | x::a' -> CSComp (CSDo (CEAssign (PreOp (ArithOp PlusOp), CEVar i,
-        CECall (len,[CEVar (n_of_int n)]))),body (n + 1) a') in
+        CECall (len,[CEVar (chars_of_int n)]))),body (n + 1) a') in
   body 1;;
 
 let args_of_format s =
   let rec args_of_format' n m =
     try if String.get s n = '%' && String.get s (n + 1) = 'd' then
-        (Some(n_of_int m),ctint_signed)::args_of_format' (n + 2) (m + 1)
+        (Some(chars_of_int m),ctint_signed)::args_of_format' (n + 2) (m + 1)
       else args_of_format' (n + 1) m
     with Invalid_argument _ -> [] in
   args_of_format' 0 1;;
@@ -308,7 +270,8 @@ let rec add_compound k0 n l =
    let k = CompoundDecl (k0,
      List.flatten (List.map (fun (t,l') -> List.map (fun f ->
        match f with
-       | ((s',t',[],_),None) -> (nindex s',ctype_of_specifier_decl_type t t')
+       | ((s',t',[],_),None) ->
+           (chars_of_string s',ctype_of_specifier_decl_type t t')
        | _ -> failwith "add_compound") l') l)) in
    try let k' = List.assoc n !the_compound_decls in
      if k' <> k then raise (Incompatible_compound (n,k',k))
@@ -346,28 +309,28 @@ and ctype_of_specifier x =
       CTInt (cint_of_specifier false None None x)
   | [Cabs.SpecType (Cabs.Tstruct (s,None,[]))] ->
       let s = name_of s in
-      CTCompound (Struct_kind,nindex s)
+      CTCompound (Struct_kind,chars_of_string s)
   | [Cabs.SpecType (Cabs.Tunion (s,None,[]))] ->
       let s = name_of s in
-      CTCompound (Union_kind,nindex s)
+      CTCompound (Union_kind,chars_of_string s)
   | [Cabs.SpecType (Cabs.Tenum (s,None,[]))] ->
       let s = name_of s in
-      CTEnum (nindex s)
+      CTEnum (chars_of_string s)
   | [Cabs.SpecType (Cabs.Tstruct (s,Some l,[]))] ->
       let s = name_of s in
-      let n = nindex s in
+      let n = chars_of_string s in
       add_compound Struct_kind n l;
       CTCompound (Struct_kind,n)
   | [Cabs.SpecType (Cabs.Tunion (s,Some l,[]))] ->
       let s = name_of s in
-      let n = nindex s in
+      let n = chars_of_string s in
       add_compound Union_kind n l;
       CTCompound (Union_kind,n)
   | [Cabs.SpecType (Cabs.Tenum (s,Some l,[]))] ->
       let s = name_of s in
-      let n = nindex s in
+      let n = chars_of_string s in
       let k = EnumDecl (int_signed,List.map (fun (s,x,_) ->
-         (nindex s,
+         (chars_of_string s,
           match x with
           | Cabs.NOTHING -> None
           | _ -> Some (cexpr_of_expression x))) l) in
@@ -375,7 +338,7 @@ and ctype_of_specifier x =
         if k' <> k then raise (Incompatible_compound (n,k',k))
       with Not_found -> the_compound_decls := !the_compound_decls@[(n,k)]);
       CTEnum n
-  | [Cabs.SpecType (Cabs.Tnamed s)] -> CTDef (nindex s)
+  | [Cabs.SpecType (Cabs.Tnamed s)] -> CTDef (chars_of_string s)
   | _ -> raise (Unknown_specifier x)
 
 and ctype_of_decl_type t x =
@@ -420,7 +383,7 @@ and cexpr_of_expression x =
      CEMax {csign = Some Signed; crank = CLongRank (nat_of_int 1)}
   | Cabs.VARIABLE "ULLONG_MAX" ->
      CEMax {csign = Some Unsigned; crank = CLongRank (nat_of_int 1)}
-  | Cabs.VARIABLE s -> CEVar (nindex s)
+  | Cabs.VARIABLE s -> CEVar (chars_of_string s)
   | Cabs.UNARY (Cabs.MEMOF,y) ->
       CEDeref (cexpr_of_expression y)
   | Cabs.UNARY (Cabs.ADDROF,y) ->
@@ -501,12 +464,13 @@ and cexpr_of_expression x =
   | Cabs.CALL (Cabs.VARIABLE "printf",
         Cabs.CONSTANT (Cabs.CONST_STRING s)::l) ->
       let fs = "printf-"^s in
-      let fresh = not (List.mem fs !the_ids) in
-      let f = nindex fs in
+      let f = chars_of_string fs in
+      let fresh =
+        try let _ = List.assoc f !the_printfs in false with Not_found -> true in
       let a = args_of_format s in
       (if fresh then (the_printfs := !the_printfs@
         [(f,if !printf_returns_int then
-           (let i = n_of_int 0 in
+           (let i = chars_of_int 0 in
             FunDecl (a,ctint_signed,
               Some (CSBlock (AutoStorage,i,ctint_signed,
                 Some (econst (Int (length_of_format s))),
@@ -515,7 +479,7 @@ and cexpr_of_expression x =
         the_formats := !the_formats@[(f,s)]));
       CECall (f,List.map cexpr_of_expression l)
   | Cabs.CALL (Cabs.VARIABLE s,l) ->
-      CECall (nindex s,List.map cexpr_of_expression l)
+      CECall (chars_of_string s,List.map cexpr_of_expression l)
   | Cabs.COMMA (h::t) ->
       List.fold_left (fun y1 y2 -> CEComma (y1,cexpr_of_expression y2))
         (cexpr_of_expression h) t
@@ -526,9 +490,9 @@ and cexpr_of_expression x =
   | Cabs.INDEX (y1,y2) ->
       CEDeref (CEBinOp (ArithOp PlusOp,
         cexpr_of_expression y1,cexpr_of_expression y2))
-  | Cabs.MEMBEROF (y,f) -> CEField (cexpr_of_expression y,nindex f)
+  | Cabs.MEMBEROF (y,f) -> CEField (cexpr_of_expression y,chars_of_string f)
   | Cabs.MEMBEROFPTR (y,f) ->
-      CEDeref (CEField (cexpr_of_expression y,nindex f))
+      CEDeref (CEField (cexpr_of_expression y,chars_of_string f))
   | Cabs.NOTHING -> econst1
   | _ -> raise (Unknown_expression x);;
 
@@ -546,7 +510,7 @@ let rec cstmt_of_statements l =
     match l with
     | [] -> cstmt_of_statements b
     | ((s,t',[],_),z)::l' ->
-        CSBlock (h,nindex s,
+        CSBlock (h,chars_of_string s,
           ctype_of_specifier_decl_type t t',
           decl_of_init_expression z,
           fold_defs h t l' b)
@@ -554,7 +518,7 @@ let rec cstmt_of_statements l =
   match l with
   | [] -> CSSkip
   | Cabs.LABEL (s,y,_)::l' ->
-      cscomp (CSLabel (nindex s,cstmt_of_statements [y]))
+      cscomp (CSLabel (chars_of_string s,cstmt_of_statements [y]))
         (cstmt_of_statements l')
   | Cabs.BLOCK ({Cabs.bstmts = y},_)::l' ->
       cscomp (cstmt_of_statements y) (cstmt_of_statements l')
@@ -590,7 +554,7 @@ let rec cstmt_of_statements l =
           cexpr_of_expression e))
         (cstmt_of_statements l')
   | Cabs.GOTO (s,_)::l' ->
-      cscomp (CSGoto (nindex s))
+      cscomp (CSGoto (chars_of_string s))
         (cstmt_of_statements l')
   | Cabs.RETURN (Cabs.NOTHING,_)::l' ->
       cscomp (CSReturn None)
@@ -621,7 +585,7 @@ let rec args_of_decl_type x =
         | (t,("",t',[],_)) ->
             (None,ctype_of_specifier_decl_type t t')
         | (t,(s,t',[],_)) ->
-            (Some(nindex s),ctype_of_specifier_decl_type t t')
+            (Some(chars_of_string s),ctype_of_specifier_decl_type t t')
         | _ -> failwith "args_of") a
   | Cabs.ARRAY (y,[],_) -> args_of_decl_type y
   | Cabs.PTR ([],y) -> args_of_decl_type y
@@ -647,9 +611,9 @@ let decls_of_definition x =
         match z with
         | ((s,t',[],_),z) ->
             (match return_of_decl_type (ctype_of_specifier t) t' with
-            | Some ret -> (nindex s, FunDecl (args_of_decl_type t', ret, None))
+            | Some ret -> (chars_of_string s, FunDecl (args_of_decl_type t', ret, None))
             | _ ->
-                (nindex s,
+                (chars_of_string s,
                  GlobDecl (ctype_of_specifier_decl_type t t',
                    decl_of_init_expression z)))
         | _ -> raise (Unknown_definition x)) l
@@ -661,7 +625,7 @@ let decls_of_definition x =
       let b = if s = "main" && no_int_return b then
         CSComp(b,CSReturn (Some (econst0))) else b in
       (match return_of_decl_type (ctype_of_specifier t) t' with
-      | Some ret -> [(nindex s, FunDecl (args_of_decl_type t', ret, Some b))]
+      | Some ret -> [(chars_of_string s, FunDecl (args_of_decl_type t', ret, Some b))]
       | None -> raise (Unknown_definition x))
   | Cabs.ONLYTYPEDEF (t,_) ->
       let _ = ctype_of_specifier t in []
@@ -669,7 +633,7 @@ let decls_of_definition x =
       List.map (fun z ->
         match z with
         | (s,t',_,_) ->
-             (nindex s,
+             (chars_of_string s,
                TypeDefDecl (ctype_of_specifier_decl_type t t'))
         | _ -> raise (Unknown_definition x)) l
   | _ -> raise (Unknown_definition x);;
@@ -677,8 +641,8 @@ let decls_of_definition x =
 let printf_prelude () =
   if !the_printfs = [] then [] else
   try let s = "len-%d" in
-    let i = n_of_int 0 and n = n_of_int 1 in
-    [(n_of_int (index s !the_ids),
+    let i = chars_of_int 0 and n = chars_of_int 1 in
+    [(chars_of_string s,
       FunDecl ([(Some i, ctint_signed)],ctint_signed,Some
        (CSBlock (AutoStorage,n,ctint_signed,Some econst0,
         CSComp (CSIf (CEBinOp (CompOp EqOp,CEVar i,econst0),
@@ -694,14 +658,13 @@ let printf_prelude () =
   with Not_found -> [];;
 
 let decls_of_cabs x =
-  the_ids := [];
   the_anon := 0;
   the_formats := [];
   the_compound_decls := [];
   the_printfs := [];
   let decls = List.flatten (List.map decls_of_definition x) in
   (the_printfs := printf_prelude ()@ !the_printfs);
-  (!the_ids,(nindex "main",!the_compound_decls@ !the_printfs@decls));;
+  (chars_of_string "main",!the_compound_decls@ !the_printfs@decls);;
 
 let decls_of_file x = decls_of_cabs (cabs_of_file x);;
 
@@ -731,7 +694,7 @@ let event_of_state x =
       with Not_found -> [])
   | _ -> [];;
 
-let initial_of_decls (_,(m,x)) =
+let initial_of_decls (m,x) =
   match interpreter_initial x86 x m [] with
   | Inl y -> raise (CH2O_error (string_of_chars y))
   | Inr y -> y;;
@@ -739,11 +702,11 @@ let initial_of_decls (_,(m,x)) =
 let initial_of_cabs x = initial_of_decls (decls_of_cabs x);;
 let initial_of_file x = initial_of_decls (decls_of_file x);;
 
-let graph_of_decls (ids,(m,x)) =
+let graph_of_decls (m,x) =
   match interpreter_all x86
     (=) event_of_state (fun x -> z_of_int (Hashtbl.hash x)) x m [] with
   | Inl y -> raise (CH2O_error (string_of_chars y))
-  | Inr y -> (ids,y);;
+  | Inr y -> y;;
 
 let graph_of_cabs x = graph_of_decls (decls_of_cabs x);;
 let graph_of_file x = graph_of_decls (decls_of_file x);;
@@ -753,15 +716,15 @@ let choose =
     then nat_of_int (Random.int (int_of_nat x))
     else nat_of_int 0);;
 
-let stream_of_decls (ids,(m,x)) =
+let stream_of_decls (m,x) =
   match interpreter_rand x86 event_of_state !choose x m [] with
   | Inl y -> raise (CH2O_error (string_of_chars y))
-  | Inr y -> (ids,y);;
+  | Inr y -> y;;
 
 let stream_of_cabs x = stream_of_decls (decls_of_cabs x);;
 let stream_of_file x = stream_of_decls (decls_of_file x);;
 
-let rec print_states ids l =
+let rec print_states l =
   match l with
   | [] -> print_string "\n"; col := 0
   | {events_all = e; sem_state = s}::l' ->
@@ -776,7 +739,7 @@ let rec print_states ids l =
            if !break_on_undef then raise (CH2O_undef y) else
            print_string "undef"
        | _ -> failwith "print_states");
-      (if l' <> [] then print_string "\n"); print_states ids l';;
+      (if l' <> [] then print_string "\n"); print_states l';;
 
 let rec string_of_events l =
   match l with
@@ -807,14 +770,14 @@ let rec find_symbol n l =
   | [(_,c)] -> c
   | (m,c)::l' -> if n <= m then c else find_symbol n l';;
 
-let trace_graph (ids,x) =
+let trace_graph x =
   let h = ref x in
   try
     while true do
       let Scons ((s1,s2),x') = Lazy.force !h in
       (if s1 = [] && s2 = [] then raise Not_found);
       (if s2 <> [] then
-        (if !col > 0 then print_string "\n"; print_states ids s2; col := 0));
+        (if !col > 0 then print_string "\n"; print_states s2; col := 0));
       (if s1 <> [] then
         let c = find_symbol (List.length s1) symbols in
         (if !col >= !trace_width then (print_string "\n"; col := 0));
@@ -836,7 +799,7 @@ let trace_decls x = trace_graph (graph_of_decls x);;
 let trace_cabs x = trace_graph (graph_of_cabs x);;
 let trace_file x = trace_graph (graph_of_file x);;
 
-let run_stream (ids,x) =
+let run_stream x =
   Random.self_init ();
   let h = ref x in
   try
