refinement_preservation.v
@@ -22,7 +22,6 @@ Ltac solve_length := simplify_equality'; repeat
 Hint Extern 0 (_ ⊑{_,_} _ : _) => refine_constructor.
 Hint Extern 0 (_ ⊑{_,_@_↦_} _ : _) => refine_constructor.
 Hint Extern 0 (_ ⊑{_,_@_↦_} _ : _ ↣ _) => refine_constructor.
-Hint Extern 0 (_\ _ ⊢ₛ _ ⇒ _) => do_cstep.
 Hint Resolve cmap_refine_memenv_refine'.
 Hint Resolve addr_alive_refine addr_strict_refine mem_writable_refine.
 Hint Resolve val_unop_ok_refine val_binop_ok_refine val_cast_ok_refine.
@@ -38,9 +37,11 @@ Hint Immediate ectx_refine_typed_l ectx_refine_typed_r.
 Hint Immediate vals_refine_typed_l vals_refine_typed_r.
 Hint Immediate locks_refine_valid_l locks_refine_valid_r.
 Hint Immediate stmt_refine_typed_l stmt_refine_typed_r.
-Hint Resolve down_refine_r up_refine_r.
+Hint Resolve direction_out_refine_r direction_in_refine_r.
+Hint Resolve sctx_item_breakto_refine.
 Hint Immediate Undef_undef.
 Hint Immediate meminj_extend_reflexive.
+Hint Immediate sctx_item_subst_refine.
 
 Lemma assign_refine_1 Γ f m1 m2 ass a1 a2 v1 v2 v1' va1' τ τ' σ :
   ✓ Γ → m1 ⊑{Γ,f} m2 → assign_typed Γ τ τ' ass σ →
@@ -219,6 +220,7 @@ Ltac invert :=
   | H : ?X ⊑{_,_@_↦_} ?Y : _ ↣ _ |- _ =>
      first [is_var X; is_var Y; fail 1|refine_inversion H]
   end.
+Ltac go f := eexists f, _; split_ands; [do_cstep| |by auto].
 Lemma cstep_refine_r Γ Γf δ1 δ2 f S1 S2 S2' g :
   ✓ Γ → Γ\ δ2 ⊢ₛ S2 ⇒ S2' → ¬is_undef_state S1 → S1 ⊑{(Γ,Γf),f} S2 : g →
   δ1 ⊑{Γ,f@'{SMem S1}↦'{SMem S2}} δ2 : Γf → ∃ f' S1',
@@ -230,19 +232,18 @@ Proof.
   destruct (cstep_preservation Γ Γf δ2 S2 S2' g) as [HS2' _];
     eauto 2 using state_refine_typed_r, funenv_refine_typed_r.
   revert Hundef HS HS2' Hδ. case p; clear p.
-  * intros m k ????; invert. exists f; eauto 10.
-  * intros m k l ????; invert. exists f; eauto 10.
-  * intros m k l ????; invert. exists f; eauto 10.
-  * intros m k E e ????; invert. exists f; eauto 11.
+  * intros m k ????; invert. go f; eauto.
+  * intros m k l ????; invert. go f; eauto.
+  * intros m k n ????; invert. go f; eauto.
+  * intros m k l ????; invert. go f; eauto.
+  * intros m k E e ????; invert. go f; eauto.
   * intros m1 m2 k E e1 e2 ?????; invert.
     edestruct ehstep_refine_r as [(f'&?&?&?&?&?&?)|[??]];
       eauto using ctx_refine_stack.
-    { eexists f', _; split_ands; auto.
-      repeat refine_constructor; eauto 10 using ctx_refine_weaken,
-         ehstep_extend, ectx_subst_refine, ectx_refine_weaken. }
-    eexists f, _; split_ands; auto. right; auto.
-    eexists; split_ands; repeat typed_constructor; eauto.
-  * intros m k h E Ωs vs ?????; invert. eexists f, _; split_ands; auto.
+    { go f'. repeat refine_constructor; eauto 9 using ctx_refine_weaken,
+       ehstep_extend, ectx_subst_refine, ectx_refine_weaken. }
+    go f. right; auto. eexists; split_ands; repeat typed_constructor; eauto.
+  * intros m k h E Ωs vs ?????; invert. go f.
     repeat refine_constructor; eauto 8 using mem_unlock_refine',
       locks_union_list_refine, ectx_refine_weaken, vals_refine_weaken,
       ctx_refine_weaken, mem_unlock_extend, option_eq_1_alt.
@@ -251,44 +252,34 @@ Proof.
         ctx_refine_stack, expr_refine_redex_inv. }
     repeat refine_constructor; eauto using mem_unlock_refine',
       expr_refine_weaken, ctx_refine_weaken, mem_unlock_extend.
-  * intros; invert. eexists f, _; split_ands; auto.
+  * intros; invert. go f.
     repeat refine_constructor; eauto using mem_unlock_extend, val_refine_weaken,
       expr_refine_weaken, ctx_refine_weaken, mem_unlock_refine'.
-  * intros; invert. eexists f, _; split_ands; auto.
+  * intros; invert. go f.
     repeat refine_constructor; eauto using mem_unlock_extend, val_refine_weaken,
       expr_refine_weaken, ctx_refine_weaken, mem_unlock_refine'.
   * intros; invert. edestruct val_true_refine_inv as [|[??]]; eauto.
-    + eexists f, _; split_ands; auto. repeat refine_constructor;
+    + go f. repeat refine_constructor;
         eauto using mem_unlock_refine', ctx_refine_weaken,
         expr_refine_weaken, stmt_refine_weaken, mem_unlock_extend.
-    + eexists f, _; split_ands; auto; right; auto.
+    + go f. right; auto.
       eexists; split_ands; eauto; repeat typed_constructor; eauto.
   * intros; invert. edestruct val_false_refine_inv as [|[??]]; eauto.
-    + eexists f, _; split_ands; auto. repeat refine_constructor;
+    + go f. repeat refine_constructor;
         eauto using mem_unlock_refine', ctx_refine_weaken,
         expr_refine_weaken, stmt_refine_weaken, mem_unlock_extend.
-    + eexists f, _; split_ands; auto; right; auto.
+    + go f. right; auto.
       eexists; split_ands; eauto; repeat typed_constructor; eauto.
-  * intros; invert. exists f; eauto 10.
-  * intros; invert. edestruct val_true_refine_inv as [|[??]]; eauto.
-    + eexists f, _; split_ands; auto. repeat refine_constructor;
-        eauto using mem_unlock_refine', ctx_refine_weaken,
-        expr_refine_weaken, stmt_refine_weaken, mem_unlock_extend.
-    + eexists f, _; split_ands; auto; right; auto.
-      eexists; split_ands; eauto; repeat typed_constructor; eauto.
-  * intros; invert. edestruct val_false_refine_inv as [|[??]]; eauto.
-    + eexists f, _; split_ands; auto. repeat refine_constructor;
-        eauto using mem_unlock_refine', ctx_refine_weaken,
-        expr_refine_weaken, stmt_refine_weaken, mem_unlock_extend.
-    + eexists f, _; split_ands; auto; right; auto.
-      eexists; split_ands; eauto; repeat typed_constructor; eauto.
-  * intros; invert. eexists f, _; split_ands; eauto 10.
-  * intros; invert. eexists f, _; split_ands; eauto 10.
-  * intros; invert. eexists f, _; split_ands; eauto 10.
-  * intros; invert. eexists f, _; split_ands; eauto 10.
-  * intros; invert. eexists f, _; split_ands; eauto 10.
-  * intros; invert. eexists f, _; split_ands; eauto 10.
-  * intros; invert. eexists f, _; split_ands; eauto.
+  * intros; invert. go f; eauto.
+  * intros; invert. go f; eauto 10.
+  * intros; invert. go f; eauto 10.
+  * intros; invert. go f; eauto 10.
+  * intros; invert. go f; eauto 10.
+  * intros; invert; go f; eauto 10.
+  * intros; invert. go f; eauto 10.
+  * intros; invert. go f; eauto 10.
+  * intros; invert. go f; eauto 10.
+  * intros; invert. go f; eauto 10.
     repeat refine_constructor; eauto. by rewrite andb_false_r.
   * intros m k h s os vs ???????; invert.
     edestruct funenv_lookup_refine_r as (?&?&?&?&?&?&?&?&?&?&?&?); eauto 2.
@@ -296,7 +287,7 @@ Proof.
     edestruct (λ m1 m2 os2 vs1, mem_alloc_val_list_refine' Γ f m1 m2
       (fresh_list (length vs1) (dom indexset m1)) os2 vs1) as (f'&?&?&?);
       eauto 2 using fresh_list_length, mem_allocable_list_fresh.
-    eexists f', _; split_ands; auto. erewrite !fmap_type_of by eauto.
+    go f'. erewrite !fmap_type_of by eauto.
     repeat refine_constructor; eauto 8 using mem_alloc_val_list_index_typed,
       mem_allocable_list_fresh, fresh_list_length,
       ctx_refine_weaken, mem_alloc_val_list_extend; simpl.
@@ -306,31 +297,31 @@ Proof.
     eauto 7 using stmt_refine_weaken, mem_alloc_val_list_refine',
       mem_alloc_val_list_extend, mem_allocable_list_fresh, fresh_list_length.
   * intros m k h oσs s ????; invert; case_match; simplify_equality'; try done.
-    eexists f, _; split_ands; auto. rewrite !fst_zip by solve_length.
+    go f. rewrite !fst_zip by solve_length.
     repeat refine_constructor; eauto using ctx_refine_weaken,
       mem_foldr_free_extend, mem_foldr_free_refine.
   * intros m k h oσs s ????; invert; case_match; simplify_equality'; try done.
-    eexists f, _; split_ands; auto. rewrite !fst_zip by solve_length.
+    go f. rewrite !fst_zip by solve_length.
     repeat refine_constructor; eauto using ctx_refine_weaken,
       val_refine_weaken, mem_foldr_free_extend, mem_foldr_free_refine.
-  * intros; invert. eexists f, _; split_ands;
-      eauto 10 using ectx_subst_refine, locks_empty_refine.
-  * intros; invert.
-    eexists f, _; split_ands; eauto 10 using sctx_item_subst_refine.
-    edestruct sctx_item_typed_Some_l; eauto using sctx_item_refine_typed_l.
-    subst; repeat refine_constructor; eauto using sctx_item_subst_refine.
-  * intros; invert. eexists f, _; split_ands; eauto.
-  * intros m k Es l s ?????; invert. exists f; eauto 10.
-  * intros m k Es l s ?????; invert.
-    exists f; eauto 10 using sctx_item_subst_refine.
+  * intros; invert. go f.
+    eauto 10 using ectx_subst_refine, locks_empty_refine.
+  * intros; invert; go f; eauto 10.
+  * intros; invert; go f; eauto 10.
+  * intros; invert; go f; eauto 10.
+  * intros; invert; go f; eauto 10.
+  * intros m k Es ??????; invert; go f. edestruct sctx_item_typed_Some_l;
+      naive_solver eauto using sctx_item_refine_typed_l.
+  * intros; invert; go f; eauto 10.
+  * intros; invert; go f; eauto 10.
   * intros m k d o τ s ??????; invert.
     edestruct (λ m1 m2 τ, mem_alloc_refine' Γ f m1 m2 false τ
       (fresh (dom _ m1))) as (f'&?&?&?); eauto 1 using mem_allocable_fresh.
-    eexists f', _; split_ands; auto. repeat refine_constructor; eauto 7 using
+    go f'. repeat refine_constructor; eauto 7 using
       mem_alloc_index_typed', direction_refine_weaken, stmt_refine_weaken,
       ctx_refine_weaken, mem_alloc_extend', mem_allocable_fresh,option_eq_1_alt.
-  * intros m k d o τ s ?????; invert.
-    eexists f, _; split_ands; auto. repeat refine_constructor; eauto 7 using
+  * intros m k d o τ s ?????; invert. go f.
+    repeat refine_constructor; eauto 7 using
       direction_refine_weaken, mem_free_refine',
       ctx_refine_weaken, mem_free_extend', option_eq_1_alt,
       index_typed_representable, index_typed_valid.
